Add Lean improvements (#2)
* `IntUtils.lean`: add proofs with `aesop`

* `EvmYulInterface`: namespace + section + aesop restructuring

* `Summaries.lean`: remove `set_option maxHeartbeats`

* `Summaries.lean`: rewrite proofs with `aesop`

* `FuncInterface`: `section` structure + `aesop` + `by rfl` -> `rfl`

* `FuncInterface`: `section` structure + proof optimization

* `StateMap.lean`: proof optimization

* `AddEquivalence.lean`: proof optimization

* `Summaries.lean`: further `by rfl` -> `rfl` and `aesop`

* `IntUtils.lean`: remove theorem `le_fls_of_lt` and unnecessary import

* `FuncInterface.lean`: more principled proofs

EvmEquivalence/Interfaces/FuncInterface.lean
@@ -17,49 +17,62 @@ namespace KEVMInterface
 
 -- Behavior for `ite`
 theorem iteMap {SortSort : Type} (c : SortBool) (x1 x2 : SortSort) :
-  kite c x1 x2  = ite c x1 x2 := by cases c <;> rfl
+  kite c x1 x2  = ite c x1 x2 := by aesop
+
+section
+
+variable {m n : SortInt}
 
 -- Behavior for `«_?Int_»`
-theorem plusIntIsSome (n m : SortInt): «_+Int_» n m = some (n + m) := by rfl
+theorem plusIntIsSome : «_+Int_» n m = some (n + m) := rfl
 
 def «_+Int'_» (n m : SortInt) : SortInt :=
-  («_+Int_» n m).get (by simp [plusIntIsSome])
+  («_+Int_» n m).get rfl
 
-theorem plusInt_def (n m : SortInt) : «_+Int'_» n m = n + m := by rfl
+theorem plusInt_def : «_+Int'_» n m = n + m := rfl
 
-theorem subIntIsSome (n m : SortInt): «_-Int_» n m = some (n - m) := by rfl
+theorem subIntIsSome : «_-Int_» n m = some (n - m) := rfl
 
 def «_-Int'_» (n m : SortInt) : SortInt :=
-  («_-Int_» n m).get (by simp [subIntIsSome])
+  («_-Int_» n m).get rfl
 
-theorem subInt_def (n m : SortInt) : «_-Int'_» n m = n - m := by rfl
+theorem subInt_def : «_-Int'_» n m = n - m := rfl
 
-theorem mulIntIsSome (n m : SortInt): «_*Int_» n m = some (n * m) := by rfl
+theorem mulIntIsSome : «_*Int_» n m = some (n * m) := rfl
 
 def «_*Int'_» (n m : SortInt) : SortInt :=
-  («_*Int_» n m).get (by simp [mulIntIsSome])
+  («_*Int_» n m).get rfl
 
-theorem mulInt_def (n m : SortInt) : «_*Int'_» n m = n * m := by rfl
+theorem mulInt_def : «_*Int'_» n m = n * m := rfl
 
 -- Behavior for `chop`
 --`_modInt_` is still uninterpreted
-theorem chopIsSome (n : SortInt) : chop n = some (n % UInt256.size) := by sorry
+theorem chopIsSome : chop n = some (n % UInt256.size) := by sorry
 
 noncomputable def chop' (n : SortInt) : SortInt :=
   (chop n).get (by simp [chopIsSome])
 
 theorem chop_def (n : SortInt) : chop' n = n % UInt256.size := by
-  simp [chop', Option.get]; split; rename_i _ _ _ _ eq _; simp_all [chopIsSome]
+  aesop (add simp [chop', chopIsSome])
+
+end
 
 -- Utils to aid in proofs
-def SortGas.val (g : SortGas) : SortInt :=
-  match g with | .inj_SortInt x => x
+def SortGas.val (g : SortGas) : SortInt := g.1
 
-theorem subGas_def (g₁ g₂ : SortGas) :
-  «_-Gas__GAS-SYNTAX_Gas_Gas_Gas»  g₁ g₂ = SortGas.inj_SortInt («_-Int'_» (SortGas.val g₁) (SortGas.val g₂)) := by rfl
+section
 
-theorem leGas_def (g₁ g₂ : SortGas) :
-  «_<=Gas__GAS-SYNTAX_Bool_Gas_Gas»  g₁ g₂ = «_<=Int_» (SortGas.val g₁) (SortGas.val g₂) := by rfl
+variable {g₁ g₂ : SortGas}
+
+theorem subGas_def :
+  «_-Gas__GAS-SYNTAX_Gas_Gas_Gas»  g₁ g₂ = SortGas.inj_SortInt («_-Int'_» (SortGas.val g₁) (SortGas.val g₂)) := rfl
+
+theorem leGas_def :
+  «_<=Gas__GAS-SYNTAX_Bool_Gas_Gas»  g₁ g₂ = «_<=Int_» (SortGas.val g₁) (SortGas.val g₂) := rfl
+
+end
+
+-- TODO: Add to a specific `axioms` namespace when enough functions have been interpreted
 
 -- Behavior of `«_==K_»` and `«_=/=K_»`
 axiom Keq_def (k₁ k₂ : SortK) : «_==K_» k₁ k₂ = some (k₁ == k₂)
@@ -75,51 +88,41 @@ axiom notBool_def (b : SortBool) : notBool_ b = some (!b)
 def wsLength (ws : SortWordStack) : ℕ :=
   match ws with
   | .«.WordStack_EVM-TYPES_WordStack» => 0
-  | .«_:__EVM-TYPES_WordStack_Int_WordStack» _ ws => 1 + wsLength ws
+  | .«_:__EVM-TYPES_WordStack_Int_WordStack» _ ws => wsLength ws + 1
 
-theorem sizeWordStackNotEmpty (n w : SortInt) (ws : SortWordStack) :
+theorem sizeWordStackNotEmpty {n w : SortInt} {ws : SortWordStack} :
   sizeWordStackAux (.«_:__EVM-TYPES_WordStack_Int_WordStack» w ws) n =
   sizeWordStackAux ws (n + 1) := by
   simp [sizeWordStackAux, _432555e, _75897fa, plusIntIsSome]
 
-theorem sizeWordStack_add_one (w : SortInt) (ws : SortWordStack) :
-  ∀ n, sizeWordStackAux (.«_:__EVM-TYPES_WordStack_Int_WordStack» w ws) n = do
+theorem sizeWordStack_add_one {w n : SortInt} {ws : SortWordStack} :
+  sizeWordStackAux (.«_:__EVM-TYPES_WordStack_Int_WordStack» w ws) n = do
   let val0 ← sizeWordStackAux ws n
   let val1 ← «_+Int_» 1 val0
   return val1 := by
-  induction ws <;> simp_all [sizeWordStackAux, _432555e, _75897fa, plusIntIsSome, Int.add_comm]
+  revert n
+  induction ws <;> simp_all [sizeWordStackAux, _432555e, _75897fa, plusIntIsSome]; introv; ring
 
-theorem sizeWordStackAuxAdd (n : SortInt) (n_nonneg: 0 ≤ n) :
-  ∀ ws, sizeWordStackAux ws (n + 1) = do
+theorem sizeWordStackAuxAdd {n : SortInt} {ws : SortWordStack} :
+  sizeWordStackAux ws (n + 1) = do
   let a ← sizeWordStackAux ws n
   let b ← «_+Int_» 1 a
   return b := by
-  cases n <;> try contradiction
-  rename_i n; cases n
-  . intro ws
-    rw [←(sizeWordStackNotEmpty (Int.ofNat 0))]
-    rw [(sizeWordStack_add_one _ ws (Int.ofNat 0))]; exact 0
-  . rename_i n ;intro ws
-    rw [←(sizeWordStackNotEmpty (Int.ofNat (n + 1)))]
-    rw [(sizeWordStack_add_one _ ws (Int.ofNat (n + 1)))]; exact 0
+  rw [←sizeWordStackNotEmpty (w := 0), sizeWordStack_add_one]
 
-theorem sizeWordStackIsSome (ws : SortWordStack) :
+theorem sizeWordStackIsSome {ws : SortWordStack} :
   «#sizeWordStack» ws = some (wsLength ws) := by
-  induction ws with
-  | «.WordStack_EVM-TYPES_WordStack» =>
-    simp [wsLength, «#sizeWordStack», _c0f9e27, sizeWordStackAux, _432555e, _75897fa]
-  | «_:__EVM-TYPES_WordStack_Int_WordStack» w wss ih =>
-    rw [«#sizeWordStack», _c0f9e27] at *
-    simp_all only [Option.pure_def, Option.bind_eq_bind, Option.bind_some]
-    rw [sizeWordStack_add_one, ih]
-    aesop
+  unfold «#sizeWordStack» _c0f9e27
+  induction' ws
+  . aesop (add simp [sizeWordStackAux, _432555e])
+  . aesop (add simp [sizeWordStack_add_one, wsLength]) (add safe (by ring))
 
-theorem wsLength_def (ws : SortWordStack) :
+theorem wsLength_eq_length_wordStackMap {ws : SortWordStack} :
   wsLength ws = List.length (wordStackMap ws) := by
-  induction ws <;> simp_all [wsLength, wordStackMap, Nat.add_comm]
+  induction ws <;> simp_all [wsLength]
 
-theorem sizeWordStack_def (ws : SortWordStack) :
-  «#sizeWordStack» ws = some (List.length (wordStackMap ws)) := by
-  rw [sizeWordStackIsSome, wsLength_def]
+theorem sizeWordStack_def {ws : SortWordStack} :
+  «#sizeWordStack» ws = some (List.length (wordStackMap ws)) :=
+  wsLength_eq_length_wordStackMap ▸ sizeWordStackIsSome
 
 end KEVMInterface
