EvmEquivalence/Interfaces/EvmYulInterface.lean
@@ -2,13 +2,21 @@ import EvmYul.UInt256
 
 open EvmYul
 
-theorem UInt256.val_eq (n : ℕ) (h : n < UInt256.size): ↑(UInt256.ofNat n).1 = n := by
-  rw [Fin.val, UInt256.val]; simp [UInt256.ofNat]; split
-  . rw [Nat.lt_iff_le_not_le] at h; cases h; contradiction
-  . simp [Id.run, Fin.ofNat]; assumption
+namespace UInt256
 
-theorem UInt256.ofNat_eq (n : ℕ) (h : n < UInt256.size):
-UInt256.ofNat n = ⟨Fin.ofNat n⟩ := by
-  simp [UInt256.ofNat]; split
-  . rw [Nat.lt_iff_le_not_le] at h; cases h; contradiction
-  . simp [Id.run]
+section
+
+set_option linter.deprecated false
+
+  variable {n : ℕ}
+
+theorem val_eq (h : n < UInt256.size): ↑(UInt256.ofNat n).1 = n := by
+  aesop (add simp [UInt256.ofNat, Id.run, Fin.ofNat])
+        (add safe (by omega))
+
+theorem ofNat_eq: UInt256.ofNat n = ⟨Fin.ofNat n⟩ := by
+  aesop (add simp [UInt256.ofNat])
+
+end
+
+end UInt256
