EvmEquivalence/StateMap.lean
@@ -79,48 +79,33 @@ def stateMap (symState : EVM.State) (tc : SortGeneratedTopCell) : EVM.State :=
 /- State Mapping Results -/
 /- Theorems to make life easier -/
 
--- This proof could be optimized
-theorem intMap_sub_dist (n m : SortInt) (le_m_n : m <= n) (pos : 0 <= m) (size : n < UInt256.size) :
+theorem intMap_sub_dist {n m : SortInt} (le_m_n : m <= n) (pos : 0 <= m) (size : n < UInt256.size) :
   intMap (n - m) = intMap n - intMap m := by
-  simp [intMap, UInt256.toSigned]; split <;> rename_i a b h
+  unfold intMap UInt256.toSigned; split <;> rename_i a b h
   . cases cn : n with
-    | ofNat p => cases cm : m with
+    | ofNat p => cases m with
                 | ofNat q =>
                 simp_all [Int.ofNat]
                 rw [←Int.ofNat_sub, Int.ofNat_inj] at h <;> try assumption
                 simp only [←h, HSub.hSub, Sub.sub, UInt256.sub, Fin.sub]
-                have size_q : q < UInt256.size := by
-                  apply (Nat.lt_of_le_of_lt le_m_n size)
-                have p_sub_q : p - q < UInt256.size := by
-                  rw [Nat.sub_lt_iff_lt_add] <;> try assumption
-                  apply Nat.lt_add_left; assumption
-                rw [UInt256.ofNat_eq] <;> try assumption
-                have eq : (UInt256.size - q + ↑(UInt256.ofNat p).1) % UInt256.size = ↑(UInt256.ofNat p).1 - q := by
-                  rw [←Nat.sub_add_comm] <;> try apply (Nat.le_of_lt size_q)
-                  rw [Nat.add_sub_assoc] <;> try rw [UInt256.val_eq] <;> try assumption
-                  rw [Nat.add_comm]; simp_arith
-                  rw [Nat.mod_eq_iff_lt]; assumption; simp [UInt256.size]
-                simp [eq, Fin.ofNat]; rw [Nat.mod_eq]
-                simp_all [UInt256.size, le_fls_of_lt, ←h, UInt256.val_eq]
-                | negSucc q => simp_all [cm]
+                aesop (add simp [UInt256.ofNat_eq, UInt256.size, Fin.ofNat])
+                      (add safe (by omega))
+                | negSucc q => aesop
     | negSucc p =>
       have _ : 0 ≤ n := by apply (Int.le_trans pos le_m_n)
-      simp_all [cn]
+      aesop
   . rw [←sub_nonneg, h] at le_m_n; contradiction
 
-theorem intMap_add_dist (n m : SortInt) (nh : 0 ≤ n) (mh : 0 ≤ m) :
+theorem intMap_add_dist {n m : SortInt} (nh : 0 ≤ n) (mh : 0 ≤ m) :
   intMap ((n + m) % ↑UInt256.size) = intMap n + intMap m := by
-  simp [intMap, UInt256.toSigned]
+  unfold intMap UInt256.toSigned
   split; rename_i h p mod_eq
   . split <;> split <;> rename_i h' q j l <;> try contradiction
-    . revert mod_eq
-      simp only [Int.ofNat_eq_coe, Int.ofNat_add_ofNat]
-      rw [Int.mod_cast, Int.toNat_ofNat, Int.ofNat_inj] <;> try simp
-      . intro mod_eq; subst mod_eq
-        simp [UInt256.ofNat, Id.run, dbgTrace]
-        congr 1; rw [Fin.add_def]; simp [←Fin.val_add]
-        simp [Fin.ofNat, Fin.add_def, UInt256.size]
-      . rw [←(Int.zero_add 0)]; apply Int.add_le_add <;> simp
+    . simp_all only [Int.ofNat_eq_coe, Int.ofNat_add_ofNat]
+      rw [Int.mod_cast, Int.toNat_ofNat, Int.ofNat_inj] at * <;> try simp
+      . aesop (add simp [UInt256.ofNat, UInt256.size, Id.run, dbgTrace, Fin.ofNat])
+              (add safe (by congr 1))
+      . aesop (add safe (by omega))
   . have mod_nonneg: 0 ≤ (n + m) % ↑UInt256.size := by
       rw [Int.mod_def']; apply Int.emod_nonneg; simp [UInt256.size]
     simp_all
