EvmEquivalence/Utils/IntUtils.lean
@@ -1,9 +1,5 @@
-import Mathlib.Order.Defs.LinearOrder
 import Mathlib.Order.Lattice
+import Aesop
 
-theorem le_fls_of_lt {n m : Nat} (h : n < m) : (m ≤ n) = False := by
-  simp [eq_iff_iff, iff_false, not_le]; assumption
-
-theorem Int.mod_cast (n m : Int) (le0n: 0 ≤ n) (le0m : 0 ≤ m):
-  n % m = ↑((Int.toNat n) % (Int.toNat m)) := by
-  simp_all [sup_of_le_left]
+theorem Int.mod_cast {n m : Int} (le0n: 0 ≤ n) (le0m : 0 ≤ m):
+  n % m = ↑((Int.toNat n) % (Int.toNat m)) := by aesop
